Add transition for unit.

SeparationLogic/Downwards2Upwards.v
@@ -17,7 +17,7 @@ Local Open Scope KripkeSemantics.
 
 Module Downwards2Upwards.
 
-Definition usSM {L: Language} {nL: NormalLanguage L} {pL: PropositionalLanguage L} {SL: SeparationLanguage L} {MD: Model} {kMD: KripkeModel MD} (M: Kmodel) {kiM: KripkeIntuitionisticModel MD M} {SA: SeparationAlgebra MD M} {dSA: DownwardsClosedSeparationAlgebra MD M} (SM: Semantics L MD) {kiSM: KripkeIntuitionisticSemantics L MD M SM} {dsSM: DownwardsSemantics L MD M SM}: @UpwardsSemantics L nL pL SL MD kMD M kiM (UpwardsClosureSA M) SM kiSM.
+Definition usSM {L: Language} {nL: NormalLanguage L} {pL: PropositionalLanguage L} {SL: SeparationLanguage L} {MD: Model} {kMD: KripkeModel MD} (M: Kmodel) {kiM: KripkeIntuitionisticModel MD M} {SA: SeparationAlgebra MD M} {dSA: DownwardsClosedSeparationAlgebra MD M} (SM: Semantics L MD) {kiSM: KripkeIntuitionisticSemantics L MD M SM} {dsSM: DownwardsSemantics L MD M SM}: @UpwardsSemantics L nL pL SL MD kMD M kiM (UpwardsClosure_SA M) SM kiSM.
 Proof.
   constructor.
   + (* sat_sepcon *)
@@ -53,7 +53,7 @@ End Downwards2Upwards.
 
 Module Downwards2Flat.
 
-Definition fsSM {L: Language} {nL: NormalLanguage L} {pL: PropositionalLanguage L} {SL: SeparationLanguage L} {MD: Model} {kMD: KripkeModel MD} (M: Kmodel) {kiM: KripkeIntuitionisticModel MD M} {SA: SeparationAlgebra MD M} {dSA: DownwardsClosedSeparationAlgebra MD M} (SM: Semantics L MD) {kiSM: KripkeIntuitionisticSemantics L MD M SM} {dsSM: DownwardsSemantics L MD M SM}: @FlatSemantics L nL pL SL MD kMD M kiM (UpwardsClosureSA M) SM kiSM.
+Definition fsSM {L: Language} {nL: NormalLanguage L} {pL: PropositionalLanguage L} {SL: SeparationLanguage L} {MD: Model} {kMD: KripkeModel MD} (M: Kmodel) {kiM: KripkeIntuitionisticModel MD M} {SA: SeparationAlgebra MD M} {dSA: DownwardsClosedSeparationAlgebra MD M} (SM: Semantics L MD) {kiSM: KripkeIntuitionisticSemantics L MD M SM} {dsSM: DownwardsSemantics L MD M SM}: @FlatSemantics L nL pL SL MD kMD M kiM (UpwardsClosure_SA M) SM kiSM.
 Proof.
   constructor.
   + (* sat_sepcon *)
