SeparationLogic/DownwardsSemantics.v
@@ -16,12 +16,7 @@ Class DownwardsSemantics (L: Language) {nL: NormalLanguage L} {pL: Propositional
   sat_wand: forall m x y, KRIPKE: M , m |= x -* y <-> forall m0 m1 m2, m0 <= m -> join m0 m1 m2 -> KRIPKE: M , m1 |= x -> KRIPKE: M, m2 |= y
 }.
 
-Class DownwardsClosedUnitarySeparationAlgebra (MD: Model) {kMD: KripkeModel MD} (M: Kmodel) {kiM: KripkeIntuitionisticModel MD M} {SA: SeparationAlgebra MD M} {USA: UnitarySeparationAlgebra MD M}: Type := {
-  unit_spec : forall m: Kworlds M, unit m <-> forall n n', join m n n' -> n' <= n;
-  unit_exists: forall n: Kworlds M, exists m, join m n n /\ (forall m', m' <= m -> unit m')
-}.
-
 Class UnitaryDownwardsSemantics (L: Language) {nL: NormalLanguage L} {pL: PropositionalLanguage L} {SL: SeparationLanguage L} {uSL: UnitarySeparationLanguage L} (MD: Model) {kMD: KripkeModel MD} (M: Kmodel) {kiM: KripkeIntuitionisticModel MD M} {SA: SeparationAlgebra MD M} {USA: UnitarySeparationAlgebra MD M} (SM: Semantics L MD) {kiSM: KripkeIntuitionisticSemantics L MD M SM} {dsSM: DownwardsSemantics L MD M SM}: Type := {
-  sat_emp: forall (m: Kworlds M), KRIPKE: M, m |= emp <-> forall n, n <= m -> unit n
+  sat_emp: forall (m: Kworlds M), KRIPKE: M, m |= emp <-> unit m
 }.
 
