SeparationLogic/SeparationAlgebra.v
@@ -16,7 +16,13 @@ Class GarbageCollectSeparationAlgebra (MD: Model) {kMD: KripkeModel MD} (M: Kmod
 }.
 
 Class UnitarySeparationAlgebra (MD: Model) {kMD: KripkeModel MD} (M: Kmodel) {kiM: KripkeIntuitionisticModel MD M} {SA: SeparationAlgebra MD M}: Type := {
-  unit: Kworlds M -> Prop
+  unit: Kworlds M -> Prop;
+  unit_spec: forall m: Kworlds M, unit m <-> forall n n', join m n n' -> n' <= n;
+  unit_exists: forall n: Kworlds M, exists m, join m n n /\ unit m
+}.
+
+Class NormalUnitarySeparationAlgebra (MD: Model) {kMD: KripkeModel MD} (M: Kmodel) {kiM: KripkeIntuitionisticModel MD M} {SA: SeparationAlgebra MD M} {USA: UnitarySeparationAlgebra MD M}: Type := {
+  unit_down: forall n m: Kworlds M, n <= m -> unit m -> unit n
 }.
 
 Class DownwardsClosedSeparationAlgebra (MD: Model) {kMD: KripkeModel MD} (M: Kmodel) {kiM: KripkeIntuitionisticModel MD M} {SA: SeparationAlgebra MD M}: Type := {
@@ -34,4 +40,15 @@ Class UpwardsClosedSeparationAlgebra (MD: Model) {kMD: KripkeModel MD} (M: Kmode
 
 It is necessary to be this strong, or else sepcon_assoc will be unsound, e.g. the following weaker version causes unsoundness:
   join_Korder: forall M (m1 m2 m n1: Kworlds M), join m1 m2 m -> Korder m1 n1 -> exists n2 n, join n1 n2 n /\ Korder m2 n2 /\ Korder m n;  *)
+
+Definition UpwardsClosed_nUSA {MD: Model} {kMD: KripkeModel MD} (M: Kmodel) {kiM: KripkeIntuitionisticModel MD M} {SA: SeparationAlgebra MD M} {uSA: UpwardsClosedSeparationAlgebra MD M} {USA: UnitarySeparationAlgebra MD M}: NormalUnitarySeparationAlgebra MD M.
+Proof.
+  constructor.
+  intros.
+  pose proof Korder_PreOrder as H_PreOrder.
+  rewrite unit_spec in H0 |- *.
+  intros.
+  destruct (join_Korder_up _ _ _ _ n0 H1 H) as [n'' [? ?]]; [reflexivity |].
+  etransitivity; eauto.
+Qed.
 
