SeparationLogic/UpwardsSemantics.v
@@ -16,11 +16,6 @@ Class UpwardsSemantics (L: Language) {nL: NormalLanguage L} {pL: PropositionalLa
   sat_wand: forall m x y, KRIPKE: M , m |= x -* y <-> forall m1 m2, join m m1 m2 -> KRIPKE: M , m1 |= x -> KRIPKE: M, m2 |= y
 }.
 
-Class UpwardsClosedUnitarySeparationAlgebra (MD: Model) {kMD: KripkeModel MD} (M: Kmodel) {kiM: KripkeIntuitionisticModel MD M} {SA: SeparationAlgebra MD M} {USA: UnitarySeparationAlgebra MD M}: Type := {
-  unit_spec : forall m: Kworlds M, unit m <-> forall n n', join m n n' -> n' <= n;
-  unit_exists: forall n: Kworlds M, exists m, join m n n /\ unit m
-}.
-
 Class UnitaryUpwardsSemantics (L: Language) {nL: NormalLanguage L} {pL: PropositionalLanguage L} {SL: SeparationLanguage L} {uSL: UnitarySeparationLanguage L} (MD: Model) {kMD: KripkeModel MD} (M: Kmodel) {kiM: KripkeIntuitionisticModel MD M} {SA: SeparationAlgebra MD M} {USA: UnitarySeparationAlgebra MD M} (SM: Semantics L MD) {kiSM: KripkeIntuitionisticSemantics L MD M SM} {usSM: UpwardsSemantics L MD M SM}: Type := {
   sat_emp: forall (m: Kworlds M), KRIPKE: M, m |= emp <-> exists n, m <= n /\ unit n
 }.
